redefine ctxRty

BaseDef.v
@@ -14,10 +14,55 @@ Definition atom_eqb_spec (s1 s2 : atom): reflect (s1 = s2) (atom_eqb s1 s2) := S
 
 From stdpp Require Import gmap.
 Definition restrict_keys {V} (s : aset) (m : amap V) : amap V :=
-  filter (λ '(k, _), (k ∈ s)) m.
+  filter (λ kx : atom * V, kx.1 ∈ s) m.
 
 Definition restrict_keys_compl {V} (s : aset) (m : amap V) : amap V :=
-  filter (λ '(k, _), (k ∉ s)) m.
+filter (λ kx : atom * V, kx.1 ∉ s) m.
+
+Lemma restrict_keys_union_compl {V} (s : aset) (m : amap V) :
+  restrict_keys s m ∪ restrict_keys_compl s m = m.
+Proof.
+  unfold restrict_keys, restrict_keys_compl.
+  rewrite (map_filter_union_complement (λ kx : atom * V, kx.1 ∈ s) m).
+  reflexivity.
+Qed.
+
+Lemma restrict_keys_split {V} (s : aset) (m : amap V) :
+  m = restrict_keys s m ∪ restrict_keys_compl s m.
+Proof. symmetry; apply restrict_keys_union_compl. Qed.
+
+Lemma dom_restrict_keys {V} (s : aset) (m : amap V) :
+  dom (restrict_keys s m) ≡ dom m ∩ s.
+Proof.
+  unfold restrict_keys.
+  eapply (dom_filter (K:=atom) (M:=amap) (D:=aset) (A:=V)
+           ).
+  intro i. split.
+  - intros H.
+    assert (i ∈ dom m) as Hs by set_solver.
+    rewrite elem_of_dom in Hs. destruct Hs as [x Hlookup].
+    exists x. split; eauto. set_solver.
+  - intros (x & Hdom & Hs).
+    assert (is_Some (m !! i)) as HSome by eauto.
+    rewrite <- elem_of_dom in HSome.
+    set_solver.
+Qed.
+
+Lemma dom_restrict_keys_compl {V} (s : aset) (m : amap V) :
+  dom (restrict_keys_compl s m) ≡ dom m ∖ s.
+Proof.
+  unfold restrict_keys_compl.
+  eapply (dom_filter (K:=atom) (M:=amap) (D:=aset) (A:=V)).
+  intro i. split.
+  - intros Hdom.
+    assert (i ∈ dom m) as Hs by set_solver.
+    rewrite elem_of_dom in Hs. destruct Hs as [x Hlookup].
+    exists x. split; eauto. set_solver.
+  - intros (x & Hdom & Hs).
+    assert (is_Some (m !! i)) as HSome by eauto.
+    rewrite <- elem_of_dom in HSome.
+    set_solver.
+Qed.
 
 Notation " '[D' s ']' " := (restrict_keys s) (at level 20, format "[D s ]", s constr).
 Notation " '[D~' s ']' " := (restrict_keys_compl s) (at level 20, format "[D~ s ]", s constr).
@@ -73,3 +118,31 @@ Class Denotation (A: Type) (B: Type) := denote: A -> B.
 Notation "'⟦' τ '⟧' " := (denote τ) (at level 20, format "⟦ τ ⟧", τ constr).
 
 Hint Unfold open close subst stale lc has_type denote amap_stale: class_simpl.
+
+Lemma stale_restrict_keys_ {V} (s : aset) (m : amap V) :
+  stale (restrict_keys s m) ≡ stale m ∩ s.
+Proof.
+  unfold stale, amap_stale.
+  rewrite dom_restrict_keys. eauto.
+Qed.
+
+Lemma stale_restrict_keys_compl_ {V} (s : aset) (m : amap V) :
+  stale (restrict_keys_compl s m) ≡ stale m ∖ s.
+Proof.
+  unfold stale, amap_stale.
+  rewrite dom_restrict_keys_compl. eauto.
+Qed.
+
+Lemma stale_restrict_keys {V} (s : aset) (m : amap V) :
+  stale (restrict_keys s m) = stale m ∩ s.
+Proof.
+  apply leibniz_equiv.
+  rewrite stale_restrict_keys_. set_solver.
+Qed.
+
+Lemma stale_restrict_keys_compl {V} (s : aset) (m : amap V) :
+  stale (restrict_keys_compl s m) = stale m ∖ s.
+Proof.
+  apply leibniz_equiv.
+  rewrite stale_restrict_keys_compl_. set_solver.
+Qed.
